Update W14.dfy

Dafny/W14.dfy
@@ -270,5 +270,115 @@ method LoopFrameExample(X: int, Y: int)
 - Loop frame are variables which are not modified inside a loop.
 - Parameters of a function can never be modified, and hence are always part of the loop frame.
 - For local variables, Dafny inspects the body and automatically determines which variables are not on the LHS of an assignment statement.
-- For arrays, programmers have to write an explicit modifies clause to indicate which array variables are modified inside the loop body.
+- For arrays, programmers have to write an explicit modifies clause to indicate which array variables would be modified.
  */
+
+method SetEndPoints(a: array<int>, left: int, right: int)
+  requires a.Length != 0
+  modifies a
+{
+  a[0] := left;
+  a[a.Length - 1] := right;
+}
+
+method EndPointCaller()
+{
+	var a := new int[10] (i => i+1);
+	assert(a[0] == 1);
+	SetEndPoints(a, 0, 0);
+	assert(a[0] == 1);    // SetEndPoints is modifying the array, so all assertions
+	assert(a[1] == 2);	  // regarding its elements will fail.
+	assert(a[0] == 0);    // The specification of SetEndPoints is not precise enough
+}
+
+method Aliases(a: array<int>, b: array<int>)
+  requires 100 <= a.Length
+  modifies a
+{
+  a[0] := 10;
+  var c := a;
+  if b == a {  
+	//Dafny is automatically able to infer that a and b are aliases here
+    b[10] := b[0] + 1;   
+  }
+  c[20] := a[14] + 2;
+}
+
+method Increment(a: array<int>, i: int)
+  requires 0 <= i < a.Length
+  modifies a
+  ensures a[i] == old(a[i]) + 1 
+  // We can use old(a[i]) refer to the value of the array element at index i at the beginning of the method, i.e. the method's pre-state
+{
+  a[i] := a[i] + 1; 
+}
+
+method InitArray(a: array<int>, d: int)
+	modifies a
+	ensures forall i :: 0 <= i < a.Length ==> a[i] == d
+{
+	var n := 0;
+	while n != a.Length
+	invariant 0 <= n <= a.Length
+	invariant forall i :: 0 <= i < n ==> a[i] == d
+	{
+		a[n] := d;
+		n := n + 1;
+	}
+}
+
+method InitArrayWithoutLoops(d: int)
+{
+	var a := new int[100] (i => d);
+	assert (forall i :: 0 <= i < a.Length ==> a[i] == d);
+}
+
+method IncrementAll(a: array<int>)
+	ensures forall i :: 0 <= i < a.Length ==> a[i] == old(a[i]) + 1
+	modifies a
+{
+	var n := 0;
+	while(n != a.Length)
+	invariant 0 <= n <= a.Length
+	invariant forall i :: 0 <= i < n ==> a[i] == old(a[i]) + 1
+	//default modifies clause of a loop is the same as the enclosing method
+	{
+		//assert(a[n] + 1 == old(a[n]) + 1);
+		a[n] := a[n] + 1;
+		//assert(forall i :: 0 <= i < n ==> a[i] == old(a[i]) + 1);
+		//assert(a[n] == old(a[n]) + 1);
+		//assert(forall i :: 0 <= i < n + 1 ==> a[i] == old(a[i]) + 1);
+		n := n + 1;
+	}
+}
+
+method IncrementAllCorrect(a: array<int>)
+	ensures forall i :: 0 <= i < a.Length ==> a[i] == old(a[i]) + 1
+	modifies a
+{
+	var n := 0;
+	while(n != a.Length)
+	invariant 0 <= n <= a.Length
+	invariant forall i :: 0 <= i < n ==> a[i] == old(a[i]) + 1
+	invariant forall i :: n <= i < a.Length ==> a[i] == old(a[i])
+	{
+		a[n] := a[n] + 1;
+		n := n + 1;
+	}
+}
+
+method Copy(src: array, dst: array)
+	modifies dst
+	requires src.Length == dst.Length
+	ensures forall i :: 0 <= i < src.Length ==> old(src[i]) == dst[i]
+{
+	var n := 0;
+	while(n != src.Length)
+	invariant 0 <= n <= src.Length
+	invariant forall i :: 0 <= i < n ==> old(src[i]) == dst[i]
+	invariant forall i :: 0 <= i < src.Length ==> old(src[i]) == src[i]
+	{
+		dst[n] := src[n];
+		n := n + 1;
+	}
+}
